formalization/Denotation.v
@@ -54,38 +54,38 @@ Notation "'⟦' τ '⟧' " := (rtyR (rty_measure τ) τ) (at level 20, format "�
 
 (** Context denotation (Fig. 7), defined as an inductive relation instead of a
   [Prop]-valued function. *)
-Inductive ctxRst: listctx rty -> pp -> Prop :=
-| ctxRst0: ctxRst [] (fun env => env = ∅)
-| ctxRst1: forall Γ pp (x: atom) b ϕ,
-    ctxRst Γ pp ->
+Inductive ctxRst: listctx rty -> epr -> Prop :=
+| ctxRst0: ctxRst [] (Epr ∅ ∅ (fun σ => σ = ∅))
+| ctxRst1: forall Γ σ L Σ (x: atom) b ϕ (v: value),
+    ctxRst Γ (Epr σ L Σ) ->
     (* [ok_ctx] implies [ρ] is closed and valid, meaning that it does not use
     any function variables. *)
     ok_ctx (Γ ++ [(x, {: b | ϕ})]) ->
-    ctxRst (Γ ++ [(x, {: b | ϕ})])
-      (fun env => exists env', pp env' /\ forall (v: value), ⟦ m{ env }r {: b | ϕ} ⟧ v -> env' = <[ x := v ]> env)
-| ctxRst2: forall Γ pp (x: atom) b ϕ,
-    ctxRst Γ pp ->
-    (* [ok_ctx] implies [ρ] is closed and valid, meaning that it does not use
-    any function variables. *)
+    ⟦ m{ σ }r {: b | ϕ} ⟧ v ->
+    ctxRst (Γ ++ [(x, {: b | ϕ})]) (Epr (<[x := v]> σ) L Σ)
+| ctxRst2: forall Γ σ L Σ (x: atom) b ϕ,
+    ctxRst Γ (Epr σ L Σ) ->
     ok_ctx (Γ ++ [(x, [: b | ϕ])]) ->
     ctxRst (Γ ++ [(x, [: b | ϕ])])
-      (fun env => exists env', pp env' /\ exists (v: value), ⟦ m{ env }r {: b | ϕ} ⟧ v /\ env' = <[ x := v ]> env)
-.
-
+      (Epr σ L (fun σ2 => exists σ1 (v: value), ⟦ m{ σ ∪ σ1 }r {: b | ϕ} ⟧ v /\ σ2 = (<[ x := v ]> σ1)))
+| ctxRst3: forall Γ σ L Σ (x: atom) ρ τ (v: value),
+    ctxRst Γ (Epr σ L Σ) ->
+    ok_ctx (Γ ++ [(x, ρ ⇨ τ)]) ->
+    ⟦ m{ σ }r (ρ ⇨ τ) ⟧ v ->
+    ctxRst (Γ ++ [(x, ρ ⇨ τ)]) (Epr (<[x := v]> σ) L Σ).
 
 (** * Properties of denotation *)
 
-Lemma langA_closed n a α β:
-  langA n a α β -> closed_td ∅ a.
-Proof.
-  destruct n; simpl; intuition.
-Qed.
-
-Lemma langA_valid_trace n a α β:
-  langA n a α β -> valid_trace α /\ valid_trace β.
-Proof.
-  destruct n; simpl; intuition.
-Qed.
+(* Lemma ctxRst_non_empty: forall Γ, (fun Γ => ok_ctx Γ -> exists P, ctxRst Γ P) Γ. *)
+(* Proof. *)
+(*   apply rev_ind. *)
+(*   - admit. *)
+(*   - intros (x & ρ) Γ HP HOk. assert (ok_ctx Γ). admit. apply HP in H. clear HP. destruct H as (P & HP). *)
+(*     destruct ρ. *)
+(*     + exists (fun Γv' => exists Γv (v: value), Γv' = (<[x := v]> Γv) /\ ⟦ m{ Γv }r {: b | ϕ} ⟧ v ). *)
+(*       econstructor; eauto. admit. *)
+(*     +  *)
+(*   induction Γ. admit. *)
 
 Lemma rtyR_typed_closed gas τ e :
   rtyR gas τ e ->
@@ -124,41 +124,38 @@ Proof.
   eauto using basic_typing_regular_tm.
 Qed.
 
-Lemma ctxRst_closed_env Γ Γv : ctxRst Γ Γv -> closed_env Γv.
-Proof.
-  unfold closed_env.
-  induction 1.
-  - apply map_Forall_empty.
-  - apply map_Forall_insert_2; eauto.
-    unfold closed_value.
-    change (fv_value v) with (fv_tm v).
-    apply equiv_empty.
-    erewrite <- dom_empty.
-    eapply basic_typing_contains_fv_tm.
-    eapply rtyR_typed_closed.
-    eauto.
-Qed.
+Lemma ctxRst_closed_pp Γ Γv : ctxRst Γ Γv -> closed_epr Γv.
+Admitted.
+(* Proof. *)
+(*   unfold close_pp. unfold closed_env. *)
+(*   induction 1; intros; subst; *)
+(*     repeat rewrite ctxdom_app_union in *; intuition; *)
+(*     try solve [apply map_Forall_empty]; *)
+(*     simpl; unfold close_pp in H1; ospecialize * H1; eauto; my_set_solver. *)
+(* Qed. *)
 
-Lemma ctxRst_lc Γ Γv :
-  ctxRst Γ Γv ->
-  map_Forall (fun _ v => lc (treturn v)) Γv.
-Proof.
-  induction 1.
-  apply map_Forall_empty.
-  apply map_Forall_insert_2; eauto.
-  apply rtyR_typed_closed in H1. simp_hyps.
-  eauto using basic_typing_regular_tm.
-Qed.
+(* Lemma ctxRst_closed_env Γ p σ L Σ : ctxRst Γ (Epr σ L Σ) -> closed_env σ. *)
+(* Proof. *)
+(*   intros. apply ctxRst_closed_pp in H. unfold close_pp in H. ospecialize * H; eauto. *)
+(*   intuition. *)
+(* Qed. *)
+
+(* Lemma ctxRst_lc Γ p Γv : *)
+(*   ctxRst Γ p -> p Γv -> *)
+(*   map_Forall (fun _ v => lc (treturn v)) Γv. *)
+(* Proof. *)
+(*   intros. apply ctxRst_closed_pp in H. unfold close_pp in H. ospecialize * H; eauto. *)
+(*   intuition. *)
+(* Qed. *)
 
 Lemma ctxRst_dom Γ Γv :
   ctxRst Γ Γv ->
-  ctxdom Γ ≡ dom Γv.
+  ctxdom Γ ≡ eprdom Γv.
 Proof.
-  induction 1; simpl; eauto.
-  rewrite ctxdom_app_union.
-  rewrite dom_insert.
-  simpl. my_set_solver.
-Qed.
+Admitted.
+(*   intros. apply ctxRst_closed_pp in H. unfold close_pp in H. ospecialize * H; eauto. *)
+(*   intuition. *)
+(* Qed. *)
 
 Lemma ctxRst_ok_ctx Γ Γv :
   ctxRst Γ Γv ->
@@ -167,22 +164,21 @@ Proof.
   induction 1; eauto. econstructor.
 Qed.
 
-Lemma ctxRst_regular Γ Γv:
-  ctxRst Γ Γv -> ok_ctx Γ /\ ctxdom Γ ≡ dom Γv /\ closed_env Γv.
-Proof.
-  pose ctxRst_ok_ctx. pose ctxRst_dom. pose ctxRst_closed_env. intuition; eauto.
-Qed.
+(* Lemma ctxRst_regular Γ p Γv: *)
+(*   ctxRst Γ p -> p Γv -> ok_ctx Γ /\ ctxdom Γ ≡ dom Γv /\ closed_env Γv. *)
+(* Proof. *)
+(*   pose ctxRst_ok_ctx. pose ctxRst_dom. pose ctxRst_closed_env. intuition; eauto. *)
+(* Qed. *)
 
-Lemma ctxRst_ok_insert Γ Γv x ρ :
-  ctxRst Γ Γv ->
-  ok_ctx (Γ ++ [(x, ρ)]) ->
-  Γv !! x = None.
-Proof.
-  inversion 2; listctx_set_simpl.
-  rewrite ctxRst_dom in * by eauto.
-  by apply not_elem_of_dom.
-Qed.
-
+(* Lemma ctxRst_ok_insert Γ p Γv x ρ : *)
+(*   ctxRst Γ p -> p Γv -> *)
+(*   ok_ctx (Γ ++ [(x, ρ)]) -> *)
+(*   Γv !! x = None. *)
+(* Proof. *)
+(*   inversion 3; listctx_set_simpl. *)
+(*   rewrite ctxRst_dom in * by eauto. *)
+(*   by apply not_elem_of_dom. *)
+(* Qed. *)
 
 Lemma mk_top_closed_rty b : closed_rty ∅ (mk_top b).
 Proof.
@@ -223,9 +219,7 @@ Lemma mk_eq_constant_over_denote_rty c:
   ⟦ mk_eq_constant_over c ⟧ c.
 Proof.
   simpl. split; [| split]; cbn; eauto using mk_eq_constant_over_closed_rty.
-  intros.
-  apply value_reduction_refl' in H.
-  destruct v; simpl in *; try hauto.
+  exists c. intuition.
 Qed.
 
 Lemma closed_base_rty_qualifier_and B ϕ1 ϕ2 Γ:
@@ -249,7 +243,8 @@ Lemma denote_base_rty_qualifier_and B ϕ1 ϕ2 ρ:
 Proof.
   intros (?&?&?) (?&?&?).
   split; [| split]; eauto using closed_base_rty_qualifier_and.
-  simp_hyps; subst. intros.
+  simp_hyps; subst.
+  exists v. intuition.
   rewrite qualifier_and_open.
   rewrite denote_qualifier_and.
   qauto.
@@ -262,7 +257,6 @@ Ltac lia_simp :=
 
 Ltac lia_tac :=
   repeat match goal with
-  | [H: _ |- context [td_measure (_ ^a^ _)] ] => rewrite <- open_preserves_td_measure
   | [H: _ |- context [rty_measure (_ ^r^ _)] ] => rewrite <- open_preserves_rty_measure
   | [H: _ |- _ <= _ ] => simpl in *; lia
   end; eauto.
@@ -273,41 +267,6 @@ Ltac exist_tac :=
       let x := fresh x in
       destruct H as (x & H); exists x; intuition
   end.
-
-Lemma langA_measure_irrelevant_aux: forall k ρ m n α β,
-    td_measure ρ <= k ->
-    k <= n ->
-    k <= m ->
-    langA n ρ α β <-> langA m ρ α β.
-Proof.
-  induction k; destruct ρ; intros m n α β Hk Hn Hm;
-    split; intro H; destruct m, n;
-    try solve [sinvert Hm; sinvert Hn; sinvert Hk; eauto];
-    try solve [lia_tac];
-    destruct H as (Hclosed & Hwfα & Hwfβ & H); simpl; intuition;
-    try solve [exist_tac; rewrite IHk; try lia_tac].
-  - left. rewrite IHk; try lia_tac.
-  - right. rewrite IHk; try lia_tac.
-  - left. rewrite IHk; try lia_tac.
-  - right. rewrite IHk; try lia_tac.
-  - rewrite IHk; try lia_tac.
-  - rewrite IHk; try lia_tac.
-Qed.
-
-Lemma langA_measure_irrelevant: forall ρ m n α β,
-    td_measure ρ <= n ->
-    td_measure ρ <= m ->
-    langA n ρ α β <-> langA m ρ α β.
-Proof.
-  intros. eapply (langA_measure_irrelevant_aux (td_measure ρ)); eauto.
-Qed.
-
-Lemma langA_measure_irrelevant' n ρ α β:
-  td_measure ρ <= n ->
-  langA n ρ α β <-> a⟦ ρ ⟧ α β.
-Proof.
-  intros. rewrite langA_measure_irrelevant; eauto.
-Qed.
 
 Lemma rty_measure_flip: forall ρ, rty_measure (flip_rty ρ) = rty_measure ρ.
 Proof.
@@ -325,17 +284,11 @@ Proof.
     try solve [sinvert Hm; sinvert Hn; sinvert Hk; eauto];
     try solve [lia_tac].
   - destruct H as (HT & Hclosed & H). simpl; intuition.
-    exist_tac. rewrite <- (IHk _ _ n); try lia_tac. rewrite <- (IHk _ _ n) in *; try lia_tac.
+    exist_tac.
+    destruct ρ1; intuition; do 2 rewrite <- (IHk _ _ n) in *; try lia_tac.
   - destruct H as (HT & Hclosed & H). simpl; intuition.
-    exist_tac. rewrite (IHk _ m); try lia_tac. rewrite (IHk _ m) in *; try lia_tac.
-  - destruct H as (HT & Hclosed & H). simpl; intuition.
-    destruct ρ; intuition.
-    + rewrite <- (IHk _ _ n) in *; try lia_tac.
-    + specialize (H α β H0). exist_tac. rewrite <- (IHk _ _ n); try lia_tac.
-  - destruct H as (HT & Hclosed & H). simpl; intuition.
-    destruct ρ; intuition.
-    + rewrite (IHk _ m) in *; try lia_tac.
-    + specialize (H α β H0). exist_tac. rewrite (IHk _ m); try lia_tac.
+    exist_tac.
+    destruct ρ1; intuition; do 2 rewrite (IHk _ m) in *; try lia_tac.
 Qed.
 
 (* The conclusion has to be strengthened to an equivalence to get around
@@ -357,17 +310,12 @@ Qed.
 
 Ltac rewrite_measure_irrelevant :=
   let t := (rewrite <- ?open_preserves_rty_measure;
-            rewrite <- ?open_preserves_td_measure;
             simpl; lia) in
   match goal with
   | H : context [rtyR _ _ _] |- _ =>
       setoid_rewrite rtyR_measure_irrelevant' in H; [ | t .. ]
   | |- context [rtyR _ _ _] =>
       setoid_rewrite rtyR_measure_irrelevant'; [ | t .. ]
-  | H : context [langA _ _ _ _] |- _ =>
-      setoid_rewrite langA_measure_irrelevant' in H; [ | t .. ]
-  | |- context [langA _ _ _ _] =>
-      setoid_rewrite langA_measure_irrelevant'; [ | t .. ]
   end.
 
 Ltac lc_solver_plus :=
@@ -382,39 +330,39 @@ Definition tm_refine e e' :=
   introduce a large set of naming lemmas about [wf_rty] (and consequently
   everything it depends on). Annoying. *)
   (exists T, ∅ ⊢t e' ⋮t T /\ ∅ ⊢t e ⋮t T) /\
-  (forall α β (v : value), α ⊧ e ↪*{ β} v -> α ⊧ e' ↪*{ β} v).
+  (forall (v : value), e ↪* v -> e' ↪* v).
 
-Definition value_refine (e e': value) :=
-  (exists T, ∅ ⊢t e' ⋮t T /\ ∅ ⊢t e ⋮t T) /\
-    (forall α β (v : value), α ⊧ e ↪*{ β} v -> α ⊧ e' ↪*{ β} v).
+(* Definition value_refine (e e': value) := *)
+(*   (exists T, ∅ ⊢t e' ⋮t T /\ ∅ ⊢t e ⋮t T) /\ *)
+(*     (forall α β (v : value), α ⊧ e ↪*{ β} v -> α ⊧ e' ↪*{ β} v). *)
 
-(* Semantic refinement preserves denotation. *)
-Lemma rtyR_refine_over b ϕ (e1 e2: value) :
-  value_refine e1 e2 ->
-  ⟦ {: b | ϕ} ⟧ e2 ->
-  ⟦ {: b | ϕ} ⟧ e1.
-Proof.
-  intros [Ht Hr]. intros. inversion H. simp_hyps; subst.
-  simpl. intuition.
-  qauto using basic_typing_tm_unique.
-Qed.
+(* (* Semantic refinement preserves denotation. *) *)
+(* Lemma rtyR_refine_over b ϕ (e1 e2: value) : *)
+(*   value_refine e1 e2 -> *)
+(*   ⟦ {: b | ϕ} ⟧ e2 -> *)
+(*   ⟦ {: b | ϕ} ⟧ e1. *)
+(* Proof. *)
+(*   intros [Ht Hr]. intros. inversion H. simp_hyps; subst. *)
+(*   simpl. intuition. *)
+(*   qauto using basic_typing_tm_unique. *)
+(* Qed. *)
 
-Lemma tm_refine_mk_app (e1 e2: tm) (v: value) T:
+Lemma tm_refine_mk_app (e1 e2 e_x: tm) T:
   tm_refine e1 e2 ->
-  lc v ->
-  ∅ ⊢t mk_app_e_v e2 v ⋮t T ->
-  tm_refine (mk_app_e_v e1 v) (mk_app_e_v e2 v).
+  lc e_x ->
+  ∅ ⊢t mk_app e2 e_x ⋮t T ->
+  tm_refine (mk_app e1 e_x) (mk_app e2 e_x).
 Proof.
   intros. destruct H as ((Te & HTe1 & HTe2) & H).
   split.
   - exists T. intuition.
-    apply mk_app_e_v_has_type_inv in H1; auto.
+    apply mk_app_has_type_inv in H1; auto.
     simp_hyps.
-    eapply mk_app_e_v_has_type; eauto. unique_basic_type. auto.
+    eapply mk_app_has_type; eauto. unique_basic_type. auto.
   - intros.
-    rewrite reduction_mk_app_e_v_f in H2 by auto.
+    rewrite reduction_mk_app_iff in H2 by auto.
     simp_hyps.
-    rewrite reduction_mk_app_e_v_f by auto.
+    rewrite reduction_mk_app_iff by auto.
     repeat eexists; eauto.
 Qed.
 
