formalization/Typing.v
@@ -2,7 +2,6 @@ From stdpp Require Import mapset.
 From CT Require Import CoreLangProp.
 From CT Require Import OperationalSemantics.
 From CT Require Import BasicTypingProp.
-From CT Require Import TransducerProp.
 From CT Require Import RefinementTypeProp.
 From CT Require Import DenotationProp.
 From CT Require Import InstantiationProp.
@@ -12,11 +11,9 @@ Import CoreLang.
 Import Tactics.
 Import NamelessTactics.
 Import ListCtx.
-Import Trace.
 Import OperationalSemantics.
 Import BasicTyping.
 Import Qualifier.
-Import Transducer.
 Import RefinementType.
 Import Denotation.
 Import Instantiation.
@@ -26,12 +23,6 @@ Import Instantiation.
   results. *)
 
 (** Well-formedness (Fig. 5) *)
-(* Definition wf_td (Γ: listctx rty) (A: transducer): Prop := closed_td (ctxdom Γ) A. *)
-
-(* Definition prefix_td (Γ: listctx rty) (A B: transducer) : Prop := *)
-(*   forall Γv, ctxRst Γ Γv -> *)
-(*         forall α, a⟦m{ Γv }a B⟧ α → *)
-(*              a⟦m{ Γv }a A ;+ ∘*⟧ α. *)
 
 (* Definition wf_rty (Γ: listctx rty) (τ: rty): Prop := closed_rty (ctxdom Γ) τ. *)
 (* | WfOver: forall Γ b ϕ, *)
@@ -48,22 +39,7 @@ Import Instantiation.
 (*     (forall x, x ∉ L -> wf_rty (Γ ++ [(x, mk_top b)]) (ρ ^p^ x)) -> *)
 (*     wf_rty Γ (b ⇢ ρ) *)
 
-(* with wf_rty: listctx rty -> rty -> Prop := *)
-(* | WfHoare: forall Γ ρ A B, *)
-(*     wf_rty Γ ρ -> *)
-(*     wf_td Γ A -> *)
-(*     wf_td Γ B -> *)
-(*     prefix_td Γ A B -> *)
-(*     wf_rty Γ (<[ A ] ρ [ B ]>) *)
-(* | WfInter: forall Γ τ1 τ2, *)
-(*     wf_rty Γ τ1 -> *)
-(*     wf_rty Γ τ2 -> *)
-(*     ⌊ τ1 ⌋ = ⌊ τ2 ⌋ -> *)
-(*     wf_rty Γ (τ1 ⊓ τ2) *)
-(* . *)
-
-Notation " Γ '⊢WF' τ " := (closed_rty (ctxdom Γ) τ) (at level 20, τ constr, Γ constr).
-Notation " Γ '⊢WFa' a " := (closed_td (ctxdom Γ) a) (at level 20, a constr, Γ constr).
+Notation " Γ '⊢WF' τ " := (closed_rty (ctxdom Γ) τ /\ is_coverage_rty τ) (at level 20, τ constr, Γ constr).
 
 Reserved Notation "Γ '⊢' e '⋮' τ"  (at level 20).
 
@@ -72,22 +48,21 @@ Reserved Notation "Γ '⊢' e '⋮' τ"  (at level 20).
 semantic subtyping in the mechanization. *)
 Definition subtyping (Γ: listctx rty) (ρ1 ρ2: rty) : Prop :=
   (* Assume [ρ1] and [ρ2] are valid [rty]s. *)
-  ⌊ ρ1 ⌋ = ⌊ ρ2 ⌋ /\ (is_tm_rty ρ1 <-> is_tm_rty ρ2) /\
-  forall Γv, ctxRst Γ Γv ->
-        forall e, ⟦m{ Γv }r ρ1⟧ e → ⟦m{ Γv }r ρ2⟧ e.
+  ⌊ ρ1 ⌋ = ⌊ ρ2 ⌋ /\ (is_coverage_rty ρ1 <-> is_coverage_rty ρ2) /\
+    forall epr, ctxRst Γ epr -> exists Γv, eprR epr Γv -> forall e, ⟦m{ Γv }r ρ1⟧ e → ⟦m{ Γv }r ρ2⟧ e.
 
 Notation " Γ '⊢' τ1 '<⋮' τ2 " := (subtyping Γ τ1 τ2) (at level 20, τ1 constr, τ2 constr, Γ constr).
 
 Definition join (Γ: listctx rty) (ρ1 ρ2 ρ3: rty) : Prop :=
   (* Assume [ρ1] and [ρ2] are valid [rty]s. *)
   ⌊ ρ1 ⌋ = ⌊ ρ2 ⌋ /\ ⌊ ρ1 ⌋ = ⌊ ρ3 ⌋ /\
-    (is_tm_rty ρ1 <-> is_tm_rty ρ2) /\ (is_tm_rty ρ1 <-> is_tm_rty ρ3) /\
-    forall Γv, ctxRst Γ Γv ->
-          forall e, ⟦m{ Γv }r ρ3⟧ e <-> ⟦m{ Γv }r ρ1⟧ e \/ ⟦m{ Γv }r ρ2⟧ e.
+    (is_coverage_rty ρ1 <-> is_coverage_rty ρ2) /\ (is_coverage_rty ρ1 <-> is_coverage_rty ρ3) /\
+    forall epr, ctxRst Γ epr -> exists Γv, eprR epr Γv ->
+                            forall e, ⟦m{ Γv }r ρ3⟧ e <-> ⟦m{ Γv }r ρ1⟧ e \/ ⟦m{ Γv }r ρ2⟧ e.
 
 Notation " Γ '⊢' τ1 '<⋮' τ2 " := (subtyping Γ τ1 τ2) (at level 20, τ1 constr, τ2 constr, Γ constr).
 
-Notation " Γ '⊢' τ1 '⋮join' τ2 '⋮=' τ3" := (join Γ τ1 τ2 τ3) (at level 20, τ1 constr, τ2 constr, τ3 constr, Γ constr).
+Notation " Γ '⊢' τ1 '⋮merge' τ2 '⋮=' τ3" := (join Γ τ1 τ2 τ3) (at level 20, τ1 constr, τ2 constr, τ3 constr, Γ constr).
 
 (* The builtin typing relation (Δ) that our type system is parameterized over. *)
 Parameter builtin_typing_relation : effop -> rty -> Prop.
@@ -113,67 +88,51 @@ where
 (** Typing rules for values and terms. Values always have refinement types, while
   terms always have Hoare automata types. *)
 Inductive term_type_check : listctx rty -> tm -> rty -> Prop :=
-| TLift: forall Γ v ρ,
-    Γ ⊢WF (ρ !<[ tdId ]>) ->
-    Γ ⊢ v ⋮v ρ ->
-    Γ ⊢ v ⋮t (ρ !<[ tdId ]>)
+| TErr: forall Γ (b: base_ty), Γ ⊢WF (mk_bot b) -> Γ ⊢ (terr b) ⋮t (mk_bot b)
+| TValue: forall Γ v τ, Γ ⊢ v ⋮v τ -> Γ ⊢ (treturn v) ⋮t τ
 | TSub: forall Γ e (τ1 τ2: rty),
     Γ ⊢WF τ2 ->
     Γ ⊢ e ⋮t τ1 ->
     Γ ⊢ τ1 <⋮ τ2 ->
     Γ ⊢ e ⋮t τ2
-| TJoin: forall Γ e (τ1 τ2 τ3: rty),
+| TMerge: forall Γ e (τ1 τ2 τ3: rty),
     Γ ⊢WF τ3 ->
     Γ ⊢ e ⋮t τ1 ->
     Γ ⊢ e ⋮t τ2 ->
-    Γ ⊢ τ1 ⋮join τ2 ⋮= τ3 ->
+    Γ ⊢ τ1 ⋮merge τ2 ⋮= τ3 ->
     Γ ⊢ e ⋮t τ3
-| TLetE: forall Γ e1 e2 ρ1 A1 τ2 A2 (L: aset),
-    (forall x, x ∉ L ->
-          (Γ ++ [(x, flip_rty ρ1)]) ⊢ (e2 ^t^ x) ⋮t (τ2 !<[ A2 ]>)) ->
-    Γ ⊢WF (τ2!<[ (ex_phi_to_td ρ1 A1) ○ A2 ]>) ->
-    Γ ⊢ e1 ⋮t (ρ1!<[ A1 ]>) ->
-    Γ ⊢ (tlete e1 e2) ⋮t (τ2!<[ (ex_phi_to_td ρ1 A1) ○ A2 ]>)
-(* | TLetEBase: forall Γ e1 e2 b1 ϕ1 A1 τ2 A2 (L: aset), *)
-(*     (forall x, x ∉ L -> *)
-(*           (Γ ++ [(x, {: b1 | ϕ1})]) ⊢ (e2 ^t^ x) ⋮t (τ2 !<[ A2 ]>)) -> *)
-(*     Γ ⊢WF (τ2!<[ (tdEx b1 ϕ1 A1) ○ A2 ]>) -> *)
-(*     Γ ⊢ e1 ⋮t ([: b1 | ϕ1]!<[ A1 ]>) -> *)
-(*     Γ ⊢ (tlete e1 e2) ⋮t (τ2!<[ (tdEx b1 ϕ1 A1) ○ A2 ]>) *)
-(* | TLetEArr: forall Γ e1 e2 ρ1 τ1 A1 τ2 A2 (L: aset), *)
-(*     (forall x, x ∉ L -> *)
-(*           (Γ ++ [(x, ρ1 ⇨ τ1)]) ⊢ (e2 ^t^ x) ⋮t (τ2 !<[ A2 ]>)) -> *)
-(*     Γ ⊢WF (τ2!<[ A1 ○ A2 ]>) -> *)
-(*     Γ ⊢ e1 ⋮t ((ρ1 ⇨ τ1) !<[ A1 ]>) -> *)
-(*     Γ ⊢ (tlete e1 e2) ⋮t (τ2!<[ A1 ○ A2 ]>) *)
-| TApp: forall Γ (v1 v2: value) e ρ2 ρ1 A1 τ2 A2 (L: aset),
-    (forall x, x ∉ L ->
-          (Γ ++ [(x, (flip_rty ρ1) ^r^ v2)]) ⊢ (e ^t^ x) ⋮t (τ2 !<[ A2 ]>)) ->
-    Γ ⊢WF (τ2!<[ ((ex_phi_to_td ρ1 A1) ^a^ v2) ○ A2 ]>) ->
-    Γ ⊢ v2 ⋮v ρ2 ->
-    Γ ⊢ v1 ⋮v (ρ2 ⇨ (ρ1!<[A1]>)) ->
-    Γ ⊢ (tletapp v1 v2 e) ⋮t (τ2!<[ ((ex_phi_to_td ρ1 A1) ^a^ v2) ○ A2 ]>)
-(* | TAppArr: forall Γ (v1 v2: value) e ρ2 ρ11 ρ12 A1 τ2 A2 (L: aset), *)
-(*     (forall x, x ∉ L -> *)
-(*           (Γ ++ [(x, (ρ11 ⇨ ρ12) ^r^ v2)]) ⊢ (e ^t^ x) ⋮t (τ2 !<[ A2 ]>)) -> *)
-(*     Γ ⊢WF (τ2!<[ (A1 ^a^ v2) ○ A2 ]>) -> *)
-(*     Γ ⊢ v2 ⋮v ρ2 -> *)
-(*     Γ ⊢ v1 ⋮v (ρ2 ⇨ ((ρ11 ⇨ ρ12)!<[A1]>)) -> *)
-(*     Γ ⊢ (tletapp v1 v2 e) ⋮t (τ2!<[ (A1 ^a^ v2) ○ A2 ]>) *)
-| TAppOp: forall Γ (op: effop) (v2: value) e ρ2 b1 ϕ1 A1 τ2 A2 (L: aset),
-    (forall x, x ∉ L ->
-          (Γ ++ [(x, {: b1 | ϕ1} ^r^ v2)]) ⊢ (e ^t^ x) ⋮t (τ2 !<[ A2 ]>)) ->
-    Γ ⊢WF (τ2!<[ ((tdEx b1 ϕ1 A1) ^a^ v2) ○ A2 ]>) ->
-    Γ ⊢ v2 ⋮v ρ2 ->
-    Γ ⊢ op ⋮o (ρ2 ⇨ ([: b1 | ϕ1]!<[A1]>)) ->
-    Γ ⊢ (tleteffop op v2 e) ⋮t (τ2!<[ ((tdEx b1 ϕ1 A1) ^a^ v2) ○ A2 ]>)
-| TMatchb: forall Γ (v: value) e1 e2 ϕ τ (L : aset),
+| TLetE: forall Γ e1 e2 τ1 τ2 (L: aset),
+    (forall x, x ∉ L -> (Γ ++ [(x, τ1)]) ⊢ (e2 ^t^ x) ⋮t τ2) ->
+    Γ ⊢WF τ2 ->
+    Γ ⊢ e1 ⋮t τ1 ->
+    Γ ⊢ (tlete e1 e2) ⋮t τ2
+| TAppOverParam: forall Γ (v1 v2: value) e b ϕ τ1 τ2 (L: aset),
+    (forall x, x ∉ L -> (Γ ++ [(x, τ1 ^r^ v2)]) ⊢ (e ^t^ x) ⋮t τ2) ->
+    Γ ⊢WF τ2 ->
+    Γ ⊢ v2 ⋮v [:b | ϕ] ->
+    Γ ⊢ v1 ⋮v ({:b | ϕ} ⇨ τ1) ->
+    Γ ⊢ (tletapp v1 v2 e) ⋮t τ2
+| TAppFuncParam: forall Γ (v1 v2: value) e ρ1 ρ2 τ1 τ2 (L: aset),
+    (forall x, x ∉ L -> (Γ ++ [(x, τ1 ^r^ v2)]) ⊢ (e ^t^ x) ⋮t τ2) ->
+    Γ ⊢WF τ2 ->
+    Γ ⊢ v2 ⋮v (ρ1 ⇨ ρ2) ->
+    Γ ⊢ v1 ⋮v ((ρ1 ⇨ ρ2) ⇨ τ1) ->
+    Γ ⊢ (tletapp v1 v2 e) ⋮t τ2
+| TAppOp: forall Γ (op: effop) (v2: value) e b ϕ b1 ϕ1 τ2 (L: aset),
+    (forall x, x ∉ L -> (Γ ++ [(x, [: b1 | ϕ1] ^r^ v2)]) ⊢ (e ^t^ x) ⋮t τ2) ->
+    Γ ⊢WF τ2 ->
+    Γ ⊢ v2 ⋮v [: b | ϕ] ->
+    Γ ⊢ op ⋮o ({: b | ϕ} ⇨ [: b1 | ϕ1]) ->
+    Γ ⊢ (tleteffop op v2 e) ⋮t τ2
+| TMatchbTrue: forall Γ (v: value) e1 e2 ϕ τ (L : aset),
     Γ ⊢WF τ ->
-    Γ ⊢ v ⋮v {:TBool | ϕ} ->
-    (* We can also directly encode the path condition without mentioning [x]: *)
-(*     {: TNat | (qual [# v] (fun V => V !!! 0 = (cbool true))%fin) & ϕ ^q^ v} *)
-    (forall x, x ∉ L -> (Γ ++ [(x, {: TBool | b0:c=true & b0:v= v & ϕ})]) ⊢ e1 ⋮t τ) ->
-    (forall x, x ∉ L -> (Γ ++ [(x, {: TBool | b0:c=false & b0:v= v & ϕ})]) ⊢ e2 ⋮t τ) ->
+    Γ ⊢ v ⋮v [:TBool | ϕ] ->
+    (forall x, x ∉ L -> (Γ ++ [(x, [: TBool | b0:c=true & b0:v= v & ϕ])]) ⊢ e1 ⋮t τ) ->
+    Γ ⊢ (tmatchb v e1 e2) ⋮t τ
+| TMatchbFalse: forall Γ (v: value) e1 e2 ϕ τ (L : aset),
+    Γ ⊢WF τ ->
+    Γ ⊢ v ⋮v [:TBool | ϕ] ->
+    (forall x, x ∉ L -> (Γ ++ [(x, [: TBool | b0:c=false & b0:v= v & ϕ])]) ⊢ e2 ⋮t τ) ->
     Γ ⊢ (tmatchb v e1 e2) ⋮t τ
 with value_type_check : listctx rty -> value -> rty -> Prop :=
 | TSubPP: forall Γ (v: value) (ρ1 ρ2: rty),
@@ -230,8 +189,8 @@ Proof.
   qauto.
 Qed.
 
-Lemma subtyping_preserves_is_tm_rty Γ τ1 τ2 :
-  Γ ⊢ τ1 <⋮ τ2 -> is_tm_rty τ1 <-> is_tm_rty τ2.
+Lemma subtyping_preserves_is_coverage_rty Γ τ1 τ2 :
+  Γ ⊢ τ1 <⋮ τ2 -> is_coverage_rty τ1 <-> is_coverage_rty τ2.
 Proof.
   qauto.
 Qed.
@@ -252,16 +211,15 @@ Proof.
   all: destruct 1; eauto.
 Qed.
 
-Lemma value_tm_typing_regular_is_tm_rty:
+Lemma value_tm_typing_regular_is_coverage_rty:
   (forall (Γ: listctx rty) (v: value) (ρ: rty),
-      Γ ⊢ v ⋮v ρ -> is_tm_rty ρ) /\
+      Γ ⊢ v ⋮v ρ -> is_coverage_rty ρ) /\
     (forall (Γ: listctx rty) (e: tm) (τ: rty),
-        Γ ⊢ e ⋮t τ -> is_tm_rty τ).
+        Γ ⊢ e ⋮t τ -> is_coverage_rty τ).
 Proof.
-  apply value_term_type_check_mutind; intros; cbn; subst; auto.
-  all: try solve [ rewrite <- subtyping_preserves_is_tm_rty; eauto].
-  sinvert H4. simp_hyps. eauto.
-  auto_pose_fv x. ospecialize * (H3 x); eauto.
+  split; intros.
+  - apply value_typing_regular_wf in H; intuition.
+  - apply tm_typing_regular_wf in H; intuition.
 Qed.
 
 Lemma value_tm_typing_regular_basic_typing:
@@ -287,25 +245,26 @@ Proof.
     eauto.
   - hauto using subtyping_preserves_basic_typing.
   - hauto using subtyping_preserves_basic_typing.
-  - destruct ρ1; simpl in *.
-    all: econstructor; eauto;
-      instantiate_atom_listctx;
-      rewrite ctx_erase_app_r in H0 by my_set_solver; eauto.
-  - destruct ρ1; simpl in *.
-    all: auto_exists_L; intros; repeat specialize_with x;
-        rewrite ctx_erase_app_r in H0 by my_set_solver;
-        simpl in H0; repeat rewrite <- rty_erase_open_eq in H0; eauto.
-  - apply effop_typing_preserves_basic_typing in H4. cbn in H4. sinvert H4.
-    econstructor; eauto. qauto.
-    instantiate_atom_listctx.
-    rewrite ctx_erase_app_r in H0 by my_set_solver.
-    rewrite <- rty_erase_open_eq in H0; eauto.
-  - auto_pose_fv x. repeat specialize_with x.
-    rewrite ctx_erase_app_r in H3, H5 by my_set_solver.
-    econstructor; eauto.
-    eapply basic_typing_strengthen_tm; eauto. my_set_solver.
-    eapply basic_typing_strengthen_tm; eauto. my_set_solver.
-Qed.
+(*   - destruct ρ1; simpl in *. *)
+(*     all: econstructor; eauto; *)
+(*       instantiate_atom_listctx; *)
+(*       rewrite ctx_erase_app_r in H0 by my_set_solver; eauto. *)
+(*   - destruct ρ1; simpl in *. *)
+(*     all: auto_exists_L; intros; repeat specialize_with x; *)
+(*         rewrite ctx_erase_app_r in H0 by my_set_solver; *)
+(*         simpl in H0; repeat rewrite <- rty_erase_open_eq in H0; eauto. *)
+(*   - apply effop_typing_preserves_basic_typing in H4. cbn in H4. sinvert H4. *)
+(*     econstructor; eauto. qauto. *)
+(*     instantiate_atom_listctx. *)
+(*     rewrite ctx_erase_app_r in H0 by my_set_solver. *)
+(*     rewrite <- rty_erase_open_eq in H0; eauto. *)
+(*   - auto_pose_fv x. repeat specialize_with x. *)
+(*     rewrite ctx_erase_app_r in H3, H5 by my_set_solver. *)
+(*     econstructor; eauto. *)
+(*     eapply basic_typing_strengthen_tm; eauto. my_set_solver. *)
+(*     eapply basic_typing_strengthen_tm; eauto. my_set_solver. *)
+(* Qed. *)
+Admitted.
 
 Lemma value_typing_regular_basic_typing: forall (Γ: listctx rty) (v: value) (ρ: rty),
     Γ ⊢ v ⋮v ρ -> ⌊ Γ ⌋* ⊢t v ⋮v ⌊ ρ ⌋.
@@ -319,97 +278,62 @@ Proof.
   apply value_tm_typing_regular_basic_typing.
 Qed.
 
-Lemma ctxRst_insert_easy Γ env (x: atom) ρ (v: value):
-    ctxRst Γ env ->
-    x ∉ ctxdom Γ ->
-    ⟦ m{ env }r ρ ⟧ v ->
-    pure_rty ρ ->
-    ctxRst (Γ ++ [(x, ρ)]) (<[ x := v ]> env).
-Proof.
-  intros. econstructor; eauto.
-  econstructor; eauto using ctxRst_ok_ctx.
-  apply rtyR_typed_closed in H1. simp_hyps.
-  (* This should be a lemma similar to [msubst_preserves_closed_rty_empty], or
-  we should strenghthen this lemma. But don't bother now as it is only used
-  here. *)
-  sinvert H3.
-  econstructor. eauto using lc_msubst_rty, ctxRst_lc.
-  rewrite fv_of_msubst_rty_closed in H5 by eauto using ctxRst_closed_env.
-  rewrite ctxRst_dom in * by eauto.
-  my_set_solver.
-Qed.
+(* Lemma ctxRst_insert_easy Γ P (x: atom) ρ P': *)
+(*     ctxRst Γ P -> *)
+(*     x ∉ ctxdom Γ -> *)
+(*     (forall env (v: value), ⟦ m{ env }r ρ ⟧ v -> P env <-> P' (<[ x := v ]> env)) -> *)
+(*     ctxRst (Γ ++ [(x, ρ)]) P'. *)
+(* Proof. *)
+(*   intros. econstructor; eauto. *)
+(*   econstructor; eauto using ctxRst_ok_ctx. *)
+(*   apply rtyR_typed_closed in H1. simp_hyps. *)
+(*   (* This should be a lemma similar to [msubst_preserves_closed_rty_empty], or *)
+(*   we should strenghthen this lemma. But don't bother now as it is only used *)
+(*   here. *) *)
+(*   sinvert H3. *)
+(*   econstructor. eauto using lc_msubst_rty, ctxRst_lc. *)
+(*   rewrite fv_of_msubst_rty_closed in H5 by eauto using ctxRst_closed_env. *)
+(*   rewrite ctxRst_dom in * by eauto. *)
+(*   my_set_solver. *)
+(* Qed. *)
 
-Lemma ctxRst_ctxfind Γ Γv x ρ :
-  ctxRst Γ Γv ->
-  ctxfind Γ x = Some ρ ->
-  fine_rty ρ ->
-  exists (v : value), Γv !! x = Some v /\ ⟦ m{ Γv }r ρ ⟧ v.
-Proof.
-  induction 1.
-  - easy.
-  - intros.
-    select (ctxfind (_ ++ _) _ = _)
-      (fun H => apply ctxfind_app in H; eauto using ok_ctx_ok).
+(* Lemma ctxRst_ctxfind Γ Γv x ρ : *)
+(*   ctxRst Γ Γv -> *)
+(*   ctxfind Γ x = Some ρ -> *)
+(*   fine_rty ρ -> *)
+(*   exists (v : value), Γv !! x = Some v /\ ⟦ m{ Γv }r ρ ⟧ v. *)
+(* Proof. *)
+(*   induction 1. *)
+(*   - easy. *)
+(*   - intros. *)
+(*     select (ctxfind (_ ++ _) _ = _) *)
+(*       (fun H => apply ctxfind_app in H; eauto using ok_ctx_ok). *)
 
-    assert (forall (v' : value), (⟦(m{env}r) ρ⟧) v' ->
-                            (⟦(m{<[x0:=v]> env}r) ρ⟧) v'). {
-      select (⟦ _ ⟧ _) (fun H => apply rtyR_typed_closed in H). simp_hyps.
-      intros.
-      apply rtyR_msubst_insert_eq; eauto using ctxRst_closed_env.
-      select (_ ⊢t _ ⋮t _)
-        (fun H => apply basic_typing_contains_fv_tm in H; simpl in H).
-      my_set_solver.
-      select (ok_ctx _) (fun H => apply ok_ctx_ok in H; apply ok_post_destruct in H).
-      srewrite ctxRst_dom.
-      simp_hyps.
-      apply not_elem_of_dom. eauto.
-    }
-    destruct_or!; simp_hyps.
-    + eexists. split; eauto.
-      assert (x <> x0). {
-        select (ok_ctx _) (fun H => sinvert H); listctx_set_simpl.
-        select (ctxfind _ _ = _) (fun H => apply ctxfind_some_implies_in_dom in H).
-        my_set_solver.
-      }
-      by simplify_map_eq.
-    + simpl in *.
-      case_decide; try easy. simplify_eq.
-      eexists. split; eauto. by simplify_map_eq.
-Qed.
-
-Lemma closed_td_comp L A B: closed_td L A○B <-> (closed_td L A /\ closed_td L B).
-Proof.
-  split; intros; intuition.
-  - sinvert H; sinvert H0. constructor; my_set_solver.
-  - sinvert H; sinvert H0. constructor; my_set_solver.
-  - sinvert H1; sinvert H0. constructor; eauto. constructor; eauto. my_set_solver.
-Qed.
-
-Lemma closed_td_ex L b ϕ A:
-  closed_td L (tdEx b ϕ A) <->
-    ((exists (L: aset), ∀ (x: atom), x ∉ L → lc_td (A ^a^ x)) /\ td_fv A ⊆ L /\ closed_rty L {:b|ϕ}).
-Proof.
-  split; intros; intuition.
-  - sinvert H. sinvert H0. econstructor; my_set_solver.
-  - sinvert H; sinvert H0. my_set_solver.
-  - sinvert H; sinvert H0. econstructor; eauto. econstructor; simpl; eauto. my_set_solver.
-  - sinvert H2. sinvert H1. simp_hyps. constructor; eauto. econstructor; eauto.
-    my_set_solver.
-Qed.
-
-Lemma langA_comp_spec: forall (A B: transducer) α β,
-    a⟦ A ○ B ⟧ α β <-> (exists α', a⟦ A ⟧ α α' /\ a⟦ B ⟧ α' β).
-Proof.
-  split; intros.
-  - simpl in *; simp_hyps.
-    eexists; eauto; intuition; repeat rewrite_measure_irrelevant; eauto.
-  - simpl in *; simp_hyps.
-    eexists; eauto; intuition; repeat rewrite_measure_irrelevant; eauto.
-    + apply langA_closed in H0. apply langA_closed in H1.
-      rewrite closed_td_comp; eauto.
-    + apply langA_valid_trace in H0; intuition.
-    + apply langA_valid_trace in H1; intuition.
-Qed.
+(*     assert (forall (v' : value), (⟦(m{env}r) ρ⟧) v' -> *)
+(*                             (⟦(m{<[x0:=v]> env}r) ρ⟧) v'). { *)
+(*       select (⟦ _ ⟧ _) (fun H => apply rtyR_typed_closed in H). simp_hyps. *)
+(*       intros. *)
+(*       apply rtyR_msubst_insert_eq; eauto using ctxRst_closed_env. *)
+(*       select (_ ⊢t _ ⋮t _) *)
+(*         (fun H => apply basic_typing_contains_fv_tm in H; simpl in H). *)
+(*       my_set_solver. *)
+(*       select (ok_ctx _) (fun H => apply ok_ctx_ok in H; apply ok_post_destruct in H). *)
+(*       srewrite ctxRst_dom. *)
+(*       simp_hyps. *)
+(*       apply not_elem_of_dom. eauto. *)
+(*     } *)
+(*     destruct_or!; simp_hyps. *)
+(*     + eexists. split; eauto. *)
+(*       assert (x <> x0). { *)
+(*         select (ok_ctx _) (fun H => sinvert H); listctx_set_simpl. *)
+(*         select (ctxfind _ _ = _) (fun H => apply ctxfind_some_implies_in_dom in H). *)
+(*         my_set_solver. *)
+(*       } *)
+(*       by simplify_map_eq. *)
+(*     + simpl in *. *)
+(*       case_decide; try easy. simplify_eq. *)
+(*       eexists. split; eauto. by simplify_map_eq. *)
+(* Qed. *)
 
 Ltac msubst_erase_simp :=
   repeat match goal with
@@ -422,24 +346,3 @@ Ltac msubst_erase_simp :=
         | context [ m{_}r _ ] => setoid_rewrite <- rty_erase_msubst_eq
         end
     end.
-
-Lemma langA_ex_spec: forall b ϕ (A: transducer) α β,
-    (a⟦tdEx b ϕ A⟧) α β <-> exists (v_x: value), (⟦{:b|ϕ}⟧) v_x /\ (a⟦A ^a^ v_x⟧) α β.
-Proof.
-  split; intros.
-  - simpl in *; simp_hyps.
-    eexists; eauto; intuition; repeat rewrite_measure_irrelevant; eauto.
-    + rewrite closed_td_ex in H. intuition.
-    + apply value_reduction_refl' in H4; sinvert H4; subst; eauto.
-  - simpl in *; simp_hyps.
-    eexists; eauto; intuition; repeat rewrite_measure_irrelevant; eauto.
-    + apply langA_closed in H1. sinvert H1. rewrite closed_td_ex. intuition.
-      * auto_exists_L. intros. assert (lc v_x) by lc_solver_plus.
-        rewrite <- subst_intro_td with (x:=x) in H3; eauto.
-        eapply lc_subst_td; eauto. my_set_solver.
-      * pose open_fv_td'. my_set_solver.
-    + apply langA_valid_trace in H1; intuition.
-    + apply langA_valid_trace in H1; intuition.
-    + exists v_x. intuition. basic_typing_solver.
-      auto_apply; eauto. intros. apply value_reduction_any_ctx. lc_solver_plus.
-Qed.
